proof/DDC/Language/SystemF2Data/Def.v
@@ -161,6 +161,14 @@ Hint Resolve getDataDef_in.
 
 
 (********************************************************************)
+(* Builtin data types must be present in the list of definitions. *)
+Definition dcUnit := DataCon   0 0. 
+Hint Unfold dcUnit.
+
+Definition tcUnit := TyConData 0 KStar.
+Hint Unfold tcUnit.
+
+
 (* Check that a definition is ok. *)
 Inductive DEFOK : list def -> def -> Prop :=
  (* Check that a data type definition is ok *)
